Coq/src/ProgES.v
@@ -1,0 +1,38 @@
+Require Import Omega Setoid Program.Basics.
+From hahn Require Import Hahn.
+From promising Require Import Basic.
+From imm Require Import Events Prog ProgToExecution.
+Require Import AuxDef.
+Require Import AuxRel.
+Require Import EventStructure.
+Require Import LblStep.
+Require Import ProgLoc.
+
+Set Implicit Arguments.
+
+Definition thread_lts (t : thread_id) : Language.t :=
+  @Language.mk
+    (list Instr.t) state
+    init
+    is_terminal
+    (ilbl_step t).
+
+Definition prog_init_threads (prog : Prog.t) :
+  IdentMap.t {lang : Language.t & Language.state lang} :=
+  IdentMap.mapi
+    (fun tid (linstr : list Instr.t) =>
+       existT _ (thread_lts tid) (ProgToExecution.init linstr))
+    prog.
+
+Definition prog_init_K (prog : Prog.t) :=
+  map
+    (fun tidc =>
+       (CInit (fst tidc), (snd tidc)))
+    (RegMap.elements
+       (prog_init_threads prog)).
+
+Definition prog_es_init (prog : Prog.t) :=
+  let loc_labs :=
+      map (fun l => Astore Xpln Opln l 0) (prog_locs prog)
+  in
+  ES.init loc_labs (prog_init_K prog).
