Coq/src/SimRel.v
@@ -14,7 +14,7 @@ Require Import EventToAction.
 Require Import LblStep.
 Require Import SimRelCont.
 Require Import SimRelEventToAction.
-(* Require Import CertRf. *)
+Require Import ProgES.
 
 Set Implicit Arguments.
 Local Open Scope program_scope.
@@ -789,7 +789,7 @@ Section SimRelLemmas.
         (PExec : program_execution prog G)
         (WF : Execution.Wf G)
         (CONS : imm_consistent G sc) : 
-    let Sinit := ES.init prog in
+    let Sinit := prog_es_init prog in
     simrel_common prog Sinit G sc (init_trav G) (ES.acts_set Sinit).
   Proof. clear S TC X. admit. Admitted.
 
