Coq/src/SimRelCertBasicStep.v
@@ -20,6 +20,7 @@ Require Import SimRelCont.
 Require Import SimRelEventToAction.
 Require Import SimRel.
 Require Import SimRelCert.
+Require Import ProgES.
 
 Set Implicit Arguments.
 Local Open Scope program_scope.
