Coq/src/SimRelStep.v
@@ -22,7 +22,8 @@ Require Import SimRelEventToAction.
 Require Import SimRel.
 Require Import SimRelCert.
 Require Import SimRelCertBasicStep.
-Require Import SimRelCertStep.  
+Require Import SimRelCertStep.
+Require Import ProgES.
 
 Set Implicit Arguments.
 Local Open Scope program_scope.
